FreeRange.lean
@@ -1,2 +1,4 @@
 import FreeRange.Range
 import FreeRange.Expr
+import FreeRange.Analyze
+import FreeRange.Soundness
